SSA/TypeClassSSA/TypeClass.lean
@@ -1,0 +1,14 @@
+structure SSA : Type 1 :=
+  ( Kind : Type )
+  ( Context : Type )
+  ( Expr : Context → Kind → Type )
+  ( Var : Context → Kind → Type )
+  ( Decl : Kind → Type )
+  ( snoc : Context → Kind → Context )
+  ( Var0 : ∀ {Γ : Context} {k : Kind}, Var (snoc Γ k) k )
+  ( VarS : ∀ {Γ : Context} {k k' : Kind}, Var Γ k → Var (snoc Γ k') k )
+  ( ret : ∀ {Γ : Context} {k : Kind}, Var Γ k → Expr Γ k )
+  ( lett : ∀ {Γ : Context} {k : Kind},  )
+
+
+
